src/program_proof/mpaxos/becomeleader_proof.v
@@ -83,10 +83,10 @@ Proof.
                   ∃ (numReplies:u64) (reply_ptrs:list loc),
                     "HnumReplies" ∷ numReplies_ptr ↦[uint64T] #numReplies ∗
                     "Hreplies_sl" ∷ is_slice_small replies_sl ptrT 1 reply_ptrs ∗
-                    "Hreplies" ∷ ([∗ list] i ↦ reply_ptr ; γsrv' ∈ reply_ptrs ; conf,
-                    ⌜reply_ptr = null⌝ ∨ (∃ reply, enterNewEpochReply.own reply_ptr reply 1 ∗
+                    "#Hreplies" ∷ ([∗ list] i ↦ reply_ptr ; γsrv' ∈ reply_ptrs ; conf,
+                    ⌜reply_ptr = null⌝ ∨ (∃ reply, readonly (enterNewEpochReply.own reply_ptr reply 1) ∗
                                               □(if decide (reply.(enterNewEpochReply.err) = (U64 0)) then
-                                                enterNewEpoch_post γsrv' reply newepoch
+                                                enterNewEpoch_post conf γ γsrv' reply newepoch
                                               else
                                                 True)
                                   ))
@@ -195,6 +195,7 @@ Proof.
         wp_pures.
         by iApply "HΦ'".
       }
+      iMod (readonly_alloc_1 with "Hreply") as "Hreply".
       wp_apply (release_spec with "[-]").
       {
         iFrame "# Hlocked".
@@ -202,10 +203,10 @@ Proof.
         iExists _, _.
         iFrame "∗".
         iApply to_named.
-        iDestruct (big_sepL2_insert_acc with "Hreplies")  as "[_ Hreplies]".
+        iDestruct (big_sepL2_insert_acc with "Hreplies")  as "[_ Hreplies2]".
         { done. }
         { done. }
-        iDestruct ("Hreplies" $! reply_ptr x2 with "[Hreply]") as "Hreplies".
+        iDestruct ("Hreplies2" $! reply_ptr x2 with "[Hreply]") as "Hreplies3".
         {
           iRight.
           iExists _.
@@ -224,7 +225,7 @@ Proof.
           symmetry.
           by apply list_insert_id.
         }
-        iFrame "Hreplies".
+        iFrame "Hreplies3".
       }
       done.
     }
@@ -273,6 +274,546 @@ Proof.
   { eauto. }
   iIntros (numSuccesses_ptr) "HnumSuccesses".
   wp_pures.
+
+  set (I:=λ (i:u64), (
+                 ∃ (W: gset nat) (latestReply_loc:loc),
+                 "%HW_in_range" ∷ ⌜∀ s, s ∈ W → s < int.nat i⌝ ∗
+                 "%HW_size_nooverflow" ∷ ⌜(size W) ≤ int.nat i⌝ ∗
+                 "HnumSuccesses" ∷ numSuccesses_ptr ↦[uint64T] #(U64 (size W)) ∗
+                 "HlatestReply_loc" ∷ latestReply_ptr ↦[ptrT] #latestReply_loc ∗
+                 if (decide (size W = 0)) then
+                   True
+                 else
+                   ∃ latestReply latestLog,
+                  "#HlatestReply" ∷ readonly (enterNewEpochReply.own latestReply_loc latestReply 1) ∗
+                  "%Hlatestlog" ∷ ⌜latestReply.(enterNewEpochReply.state) = get_state latestLog⌝ ∗
+                  "%HlatestlogLen" ∷ ⌜int.nat latestReply.(enterNewEpochReply.nextIndex) = length latestLog⌝ ∗
+                  "%HlatestEpoch_ineq" ∷ ⌜int.nat latestReply.(enterNewEpochReply.acceptedEpoch) < int.nat newepoch⌝ ∗
+                  "#Hlatest_prop_lb" ∷ is_proposal_lb γ latestReply.(enterNewEpochReply.acceptedEpoch) latestLog ∗
+                  "#Hacc_lbs" ∷ (□ [∗ list] s ↦ γsrv' ∈ conf, ⌜s ∈ W⌝ →
+                                        is_accepted_upper_bound γsrv' latestLog
+                                                                latestReply.(enterNewEpochReply.acceptedEpoch)
+                                                                newepoch
+                                )
+      )%I).
+
+  wp_apply (wp_forSlice (V:=loc) I _ _ _ _ _ reply_ptrs with "[] [HnumSuccesses HlatestReply Hreplies_sl]").
+  2: {
+    iFrame "Hreplies_sl".
+    iExists ∅, null.
+    rewrite size_empty.
+    simpl.
+    iFrame.
+    done.
+  }
+  { (* one iteration of loop *)
+    clear Φ.
+    iIntros (?? Φ) "!# (Hi & %Hi_lt & %Hi_lookup) HΦ".
+    iNamed "Hi".
+    wp_pures.
+    wp_if_destruct.
+    {
+      iDestruct (big_sepL2_lookup_1_some with "Hreplies") as (?) "%Hi_conf_lookup".
+      { done. }
+      iDestruct (big_sepL2_lookup_acc with "Hreplies") as "[#Hreply_post _]".
+      { done. }
+      { done. }
+      iDestruct "Hreply_post" as "[%Hbad|#Hreply_post]".
+      {
+        exfalso. rewrite Hbad in Heqb1. done.
+      }
+      iDestruct "Hreply_post" as (?) "[#Hreply Hpost]".
+      iMod (readonly_load with "Hreply") as (?) "Hreplyq".
+      iNamed "Hreplyq".
+      wp_loadField.
+      wp_if_destruct.
+      { (* got ENone, increase size of W *)
+        wp_load.
+        wp_if_destruct.
+        { (* this is the first successful reply, no need to compare with other replies *)
+          wp_store.
+          wp_pures.
+          wp_load.
+          wp_store.
+          replace (W) with (∅:gset nat); last first.
+          {
+            admit. (* TODO: pure proof, size of gset = 0 → gset is ∅ *)
+          }
+          iModIntro.
+          iApply "HΦ".
+
+          iExists {[ int.nat i ]}, x.
+          iSplitR.
+          {
+            iPureIntro.
+            intros.
+            apply elem_of_singleton_1 in H.
+            rewrite H.
+            word.
+          }
+          iSplitR.
+          {
+            iPureIntro.
+            rewrite size_singleton.
+            word.
+          }
+          iFrame.
+          rewrite size_singleton.
+          rewrite size_empty.
+          iFrame.
+          simpl.
+          rewrite Heqb.
+          iDestruct "Hpost" as "#Hpost".
+          destruct (decide (_)); last first.
+          { exfalso. done. }
+          iDestruct "Hpost" as (?) "(%Hepoch_ineq & %Hlog & %Hlen & #Hacc_ub & #Hprop_lb & #Hprop_facts)".
+          iExists reply, log.
+          iFrame "Hreply".
+          iFrame "#%".
+          iModIntro.
+          iApply big_sepL_forall.
+          iIntros.
+          replace (x0) with (x2); last first.
+          {
+            apply elem_of_singleton_1 in H0.
+            rewrite H0 in H.
+            rewrite H in Hi_conf_lookup.
+            by injection Hi_conf_lookup.
+          }
+          iFrame "#".
+        }
+        { (* In this case, there have been previous successful replies. Compare with latestReply *)
+          wp_load.
+          destruct (decide (size W = 0)).
+          { exfalso. rewrite e in Heqb2. done. }
+          iNamed "Hi".
+          iMod (readonly_load with "HlatestReply") as (?) "HlatestReply2".
+          iRename "Hreply_acceptedEpoch" into "Hreply_acceptedEpoch2".
+          iRename "Hreply_nextIndex" into "Hreply_nextIndex2".
+          iClear "Hreply_err Hreply_ret Hreply_ret_sl".
+          iNamed "HlatestReply2".
+          wp_loadField.
+          wp_loadField.
+          wp_if_destruct.
+          { (* case: newreply.acceptedEpoch > latestReply.acceptedEpoch *)
+            wp_store.
+            wp_pures.
+            wp_load.
+            wp_store.
+            iModIntro.
+            iApply "HΦ".
+
+            iExists (W ∪ {[ int.nat i ]}), x.
+
+            iSplitR.
+            {
+              iPureIntro.
+              intros.
+              apply elem_of_union in H as [H|H].
+              {
+                specialize (HW_in_range s0 H).
+                word.
+              }
+              {
+                rewrite elem_of_singleton in H.
+                word.
+              }
+            }
+            rewrite size_union; last first.
+            {
+              apply disjoint_singleton_r.
+              destruct (decide (int.nat i ∈ W)).
+              {
+                exfalso.
+                specialize (HW_in_range (int.nat i) e).
+                word.
+              }
+              done.
+            }
+            rewrite size_singleton.
+            iSplitR.
+            {
+              iPureIntro.
+              word.
+            }
+            replace (word.add (size W) 1) with (U64 (size W + 1)%nat) by word.
+            iFrame.
+            destruct (decide (size W + 1 = 0)).
+            { done. }
+
+            iDestruct "Hpost" as "#Hpost".
+            destruct (decide (_)); last first.
+            { exfalso. done. }
+            iDestruct "Hpost" as (?) "(%Hepoch_ineq & %Hlog & %Hlen & #Hacc_ub & #Hprop_lb & #Hprop_facts)".
+            iExists reply, log.
+            iFrame "Hreply Hprop_lb %".
+            iModIntro.
+            iApply (big_sepL_impl with "Hacc_lbs").
+            iModIntro.
+            iIntros (???) "#Hwand".
+            iIntros "%Hin".
+
+            rewrite elem_of_union in Hin.
+            destruct Hin as [Hold|Hnew].
+            {
+              iSpecialize ("Hwand" with "[%//]").
+              iFrame.
+              iDestruct (is_accepted_upper_bound_mono_epoch with "Hwand") as "Hwand2".
+              { instantiate (1:=reply.(enterNewEpochReply.acceptedEpoch)). word. }
+              { done. }
+              iDestruct (is_accepted_upper_bound_mono_log with "Hwand2") as "$".
+              { apply prefix_nil. }
+            }
+            {
+              rewrite elem_of_singleton in Hnew.
+              rewrite Hnew.
+              replace (x2) with (x0).
+              { iFrame "Hacc_ub". }
+              rewrite Hnew in H.
+              rewrite H in Hi_conf_lookup.
+              by injection Hi_conf_lookup.
+            }
+          }
+          { (* *)
+            wp_load.
+            wp_loadField.
+            wp_loadField.
+            wp_pures.
+            destruct (bool_decide _) as [] eqn:X.
+            { (* case: same epoch *)
+              wp_pures.
+              wp_load.
+              wp_loadField.
+              wp_loadField.
+              wp_if_destruct.
+              { (* reply has higher nextIndex than latestReply *)
+                wp_store.
+                wp_load.
+                wp_store.
+                iModIntro.
+                iApply "HΦ".
+
+                (* establish loop invariant *)
+                iExists (W ∪ {[ int.nat i ]}), x.
+                iSplitR.
+                {
+                  iPureIntro.
+                  intros.
+                  apply elem_of_union in H as [H|H].
+                  {
+                    specialize (HW_in_range s0 H).
+                    word.
+                  }
+                  {
+                    rewrite elem_of_singleton in H.
+                    word.
+                  }
+                }
+                rewrite size_union; last first.
+                {
+                  apply disjoint_singleton_r.
+                  destruct (decide (int.nat i ∈ W)).
+                  {
+                    exfalso.
+                    specialize (HW_in_range (int.nat i) e).
+                    word.
+                  }
+                  done.
+                }
+                rewrite size_singleton.
+                iSplitR.
+                {
+                  iPureIntro.
+                  word.
+                }
+                replace (word.add (size W) 1) with (U64 (size W + 1)%nat) by word.
+                iFrame.
+                destruct (decide (size W + 1 = 0)).
+                { done. }
+
+                iDestruct "Hpost" as "#Hpost".
+                destruct (decide (_)); last first.
+                { exfalso. done. }
+                iDestruct "Hpost" as (?) "(%Hepoch_ineq & %Hlog & %Hlen & #Hacc_ub & #Hprop_lb & #Hprop_facts)".
+                iExists reply, log.
+                iFrame "Hreply Hprop_lb %".
+                iModIntro.
+                iApply (big_sepL_impl with "Hacc_lbs").
+                iModIntro.
+                iIntros (???) "#Hwand".
+                iIntros "%Hin".
+
+                rewrite elem_of_union in Hin.
+                destruct Hin as [Hold|Hnew].
+                {
+                  iSpecialize ("Hwand" with "[%//]").
+                  iFrame.
+                  rewrite X.
+                  iDestruct (is_proposal_lb_compare with "Hprop_lb Hlatest_prop_lb") as "%Hpre".
+                  {
+                    word.
+                  }
+                  iDestruct (is_accepted_upper_bound_mono_log with "Hwand") as "$".
+                  { done. }
+                }
+                {
+                  rewrite elem_of_singleton in Hnew.
+                  rewrite Hnew.
+                  replace (x2) with (x0).
+                  { iFrame "Hacc_ub". }
+                  rewrite Hnew in H.
+                  rewrite H in Hi_conf_lookup.
+                  by injection Hi_conf_lookup.
+                }
+              }
+              { (* keep the old latestReply *)
+                wp_pures.
+                wp_load.
+                wp_store.
+                iModIntro.
+                iApply "HΦ".
+
+                (* establish loop invariant *)
+                iExists (W ∪ {[ int.nat i ]}), _.
+                iSplitR.
+                {
+                  iPureIntro.
+                  intros.
+                  apply elem_of_union in H as [H|H].
+                  {
+                    specialize (HW_in_range s0 H).
+                    word.
+                  }
+                  {
+                    rewrite elem_of_singleton in H.
+                    word.
+                  }
+                }
+                rewrite size_union; last first.
+                {
+                  apply disjoint_singleton_r.
+                  destruct (decide (int.nat i ∈ W)).
+                  {
+                    exfalso.
+                    specialize (HW_in_range (int.nat i) e).
+                    word.
+                  }
+                  done.
+                }
+                rewrite size_singleton.
+                iSplitR.
+                {
+                  iPureIntro.
+                  word.
+                }
+                replace (word.add (size W) 1) with (U64 (size W + 1)%nat) by word.
+                iFrame.
+                destruct (decide (size W + 1 = 0)).
+                { done. }
+                iExists _, _; iFrame "#%".
+
+                iDestruct "Hpost" as "#Hpost".
+                destruct (decide (_)); last first.
+                { exfalso. done. }
+                iDestruct "Hpost" as (?) "(%Hepoch_ineq & %Hlog & %Hlen & #Hacc_ub & #Hprop_lb & #Hprop_facts)".
+                iModIntro.
+                iApply (big_sepL_impl with "Hacc_lbs").
+                iModIntro.
+                iIntros (???) "#Hwand".
+                iIntros "%Hin".
+
+                rewrite elem_of_union in Hin.
+                destruct Hin as [Hold|Hnew].
+                {
+                  iSpecialize ("Hwand" with "[%//]").
+                  iFrame.
+                  done.
+                }
+                {
+                  rewrite elem_of_singleton in Hnew.
+                  rewrite Hnew.
+                  rewrite X.
+
+                  iDestruct (is_proposal_lb_compare with "Hlatest_prop_lb Hprop_lb") as %Hpre.
+                  {
+                    word.
+                  }
+                  replace (x0) with (x2).
+                  {
+                    iDestruct (is_accepted_upper_bound_mono_log with "Hacc_ub") as "$".
+                    done.
+                  }
+                  rewrite Hnew in H.
+                  rewrite H in Hi_conf_lookup.
+                  by injection Hi_conf_lookup.
+                }
+              }
+            }
+            (* case: epoch is not the same, so keep the old latest reply *)
+            wp_pures.
+            wp_load.
+            wp_store.
+            iModIntro.
+            iApply "HΦ".
+
+            (* establish loop invariant *)
+            iExists (W ∪ {[ int.nat i ]}), _.
+            iSplitR.
+            {
+              iPureIntro.
+              intros.
+              apply elem_of_union in H as [H|H].
+              {
+                specialize (HW_in_range s0 H).
+                word.
+              }
+              {
+                rewrite elem_of_singleton in H.
+                word.
+              }
+            }
+            rewrite size_union; last first.
+            {
+              apply disjoint_singleton_r.
+              destruct (decide (int.nat i ∈ W)).
+              {
+                exfalso.
+                specialize (HW_in_range (int.nat i) e).
+                word.
+              }
+              done.
+            }
+            rewrite size_singleton.
+            iSplitR.
+            {
+              iPureIntro.
+              word.
+            }
+            replace (word.add (size W) 1) with (U64 (size W + 1)%nat) by word.
+            iFrame.
+            destruct (decide (size W + 1 = 0)).
+            { done. }
+            iExists _, _; iFrame "#%".
+
+            iDestruct "Hpost" as "#Hpost".
+            destruct (decide (_)); last first.
+            { exfalso. done. }
+            iDestruct "Hpost" as (?) "(%Hepoch_ineq & %Hlog & %Hlen & #Hacc_ub & #Hprop_lb & #Hprop_facts)".
+            iModIntro.
+            iApply (big_sepL_impl with "Hacc_lbs").
+            iModIntro.
+            iIntros (???) "#Hwand".
+            iIntros "%Hin".
+
+            rewrite elem_of_union in Hin.
+            destruct Hin as [Hold|Hnew].
+            {
+              iSpecialize ("Hwand" with "[%//]").
+              iFrame.
+              done.
+            }
+            {
+              rewrite elem_of_singleton in Hnew.
+              rewrite Hnew.
+
+              replace (x0) with (x2).
+              {
+                rewrite bool_decide_eq_false in X.
+                iDestruct (is_accepted_upper_bound_mono_epoch with "Hacc_ub") as "Hacc_ub2".
+                {
+                  instantiate (1:=latestReply.(enterNewEpochReply.acceptedEpoch)).
+                  destruct (decide (int.nat reply.(enterNewEpochReply.acceptedEpoch) = int.nat latestReply.(enterNewEpochReply.acceptedEpoch))).
+                  {
+                    exfalso.
+                    replace (reply.(enterNewEpochReply.acceptedEpoch)) with (latestReply.(enterNewEpochReply.acceptedEpoch)) in X by word.
+                    done.
+                  }
+                  word.
+                }
+                { done. }
+                iDestruct (is_accepted_upper_bound_mono_log with "Hacc_ub2") as "$".
+                { apply prefix_nil. }
+              }
+              rewrite Hnew in H.
+              rewrite H in Hi_conf_lookup.
+              by injection Hi_conf_lookup.
+            }
+          }
+        }
+      }
+      { (* got error, don't change anything *)
+        iModIntro.
+        iApply "HΦ".
+        iExists W, _.
+        iFrame "∗#%".
+        iPureIntro.
+        replace (int.nat (word.add i 1%Z)) with (int.nat i + 1) by word.
+        split.
+        {
+          intros.
+          specialize (HW_in_range s0 H).
+          word.
+        }
+        {
+          word.
+        }
+      }
+    }
+    { (* null pointer, don't do anything *)
+      iModIntro.
+      iApply "HΦ".
+      iExists W, _.
+      iFrame "∗#%".
+      iPureIntro.
+      replace (int.nat (word.add i 1%Z)) with (int.nat i + 1) by word.
+      split.
+      {
+        intros.
+        specialize (HW_in_range s0 H).
+        word.
+      }
+      {
+        word.
+      }
+    }
+  }
+  iIntros "[Hi _]".
+  wp_pures.
+  iNamed "Hi".
+  wp_load.
+  wp_if_destruct.
+  {
+    wp_loadField.
+    destruct (decide (size W = 0)).
+    {
+      exfalso.
+      rewrite e in Heqb1.
+      admit. (* FIXME: derive contradiction from X < 0 *)
+    }
+
+    wp_apply (acquire_spec with "HmuInv").
+    iIntros "[Hlocked2 Hown]".
+    wp_pures.
+    iNamed "Hown".
+    wp_loadField.
+    wp_loadField.
+    wp_if_destruct.
+    {
+      wp_loadField.
+      wp_storeField.
+      wp_storeField.
+      wp_loadField.
+      wp_storeField.
+      wp_load.
+
+      iNamed "Hi".
+      admit.
+    }
+    {
+      wp_pures.
+      wp_loadField.
+      admit.
+    }
 Admitted.
 
 End becomeleader_proof.
